fixed lem_inv_g_a_iv_f_check_for_next_queued_duty; added f_wrap_DVCState_with_Outputs

src/proofs/common/helper_pred_fcn.dfy
@@ -250,4 +250,10 @@ module Helper_Pred_Fcn
         );
         ret_process
     }   
+
+    predicate latest_att_duty_and_nonempty_duty_queue(s: DVCState) 
+    {
+        && |s.attestation_duties_queue| > 0 
+        && s.latest_attestation_duty.isPresent()  
+    }
 }
